

1) show $m(a + bX) = a + bm(X)$

$$m(a + bX) = \frac{1}{N} \sum_{i=1}^N (a + bx_i)$$

$$= \frac{1}{N} \left(\sum_{i=1}^N a + b \sum_{i=1}^N x_i \right)$$

$$= \frac{1}{N} (Na) + b \left(\frac{1}{N} \sum_{i=1}^N x_i \right)$$

$$= a + bm(X)$$

2) show $\text{cov}(X, X) = S^2$

$$\text{cov}(X, X) = \frac{1}{N} \sum_{i=1}^N (x_i - m(X))(x_i - m(X))$$

$$= \frac{1}{N} \sum_{i=1}^N (x_i - m(X))^2 = S^2$$

3) show $\text{cov}(X, a + bY) = b \text{cov}(X, Y)$

$$\star m(a + bY) = a + bm(Y)$$

$$\text{cov}(X, a + bY) = \frac{1}{N} \sum_{i=1}^N (x_i - m(X))((a + by_i) - m(a + bY))$$

$$= \frac{1}{N} \sum_{i=1}^N (x_i - m(X))(a + by_i - (a + bm(Y)))$$

$$= \frac{1}{N} \sum_{i=1}^N (x_i - m(X)) \cdot b(y_i - m(Y))$$

$$= b \left(\frac{1}{N} \sum_{i=1}^N (x_i - m(X))(y_i - m(Y)) \right)$$

$$= b \operatorname{cov}(X, Y)$$

4) show that $\operatorname{cov}(a + bX, a + bY) = b^2 \operatorname{cov}(X, Y)$

Since

$$(a + bx_i) - m(a + bX) = b(x_i - m(X))$$

$$(a + by_i) - m(a + bY) = b(y_i - m(Y))$$

so

$$\operatorname{cov}(a + bX, a + bY) = \frac{1}{N} \sum_{i=1}^N b(x_i - m(X)) \cdot b(y_i - m(Y))$$

$$= b^2 \operatorname{cov}(X, Y)$$

$$\operatorname{cov}(bX, bX) = b^2 \operatorname{cov}(X, X) = b^2 \sigma^2$$

5)

Yes, if $b > 0$, $a + bX$ is increasing, so it preserves order.
The median will shift accordingly.

$$\text{med}(a + bX) = a + b\text{med}(X)$$

The quartiles will shift the same way.

$$\begin{aligned} IQR(a + bX) &= (Q3_{a+bX} - Q1_{a+bX}) \\ &= (a + bQ3_X) - (a + bQ1_X) \\ &= bIQR(X) \end{aligned}$$

b) Let $P(X=0) = 0.5$, $P(X=4) = 0.5$

$$m(X) = 0 + 2 = 2$$

$$(m(X))^2 = 2^2 = 4$$

$$m(X^2) = E[X^2] = 0 + 8 = 8$$

$$8 \neq 4 = (m(X))^2$$

$$\sqrt{m(X)} = \sqrt{2}$$

$$m(\sqrt{X}) = E[\sqrt{X}] = 0 + 1 = 1$$

$$m(\sqrt{X}) = 1 \neq \sqrt{2} = \sqrt{m(X)}$$